Update SkipList2.Addition.fst

SkipList2/SkipList2.Addition.fst
@@ -114,6 +114,49 @@ let shiftSequence sequence_init i value=
     let temp = (Seq.append first_part second_part) in 
     Seq.append temp third_part
 
+
+(*let rec sorted #a f s =
+  if length s <= 1
+  then true *)
+
+(*abstract val slice:  #a:Type -> s:seq a -> i:nat -> j:nat{i <= j && j <= length s} -> Tot (seq a) (decreases (length s)
+val slice_lemma : #a: eqtype -> #f:(cmp a) -> sequence_init : seq a {Seq.sorted f sequence_init}
+-> i: nat {0<= i &&  i <= Seq.length sequence_init}  -> 
+        Lemma(ensures (Seq.sorted f (Seq.slice sequence_init i (Seq.length sequence_init))))
+        (decreases (Seq.slice sequence_init )) 
+
+let rec slice_lemma #a #f sequence_init i = 
+    match i with 
+    0 -> () 
+    | _ -> let i = i + 1 in if i = Seq.length sequence_init then () else slice_lemma sequence_init i+1
+
+*)
+(*)
+val test: #a : eqtype -> #f: (a -> a -> Tot bool)  -> sequence_init : seq a{Seq.sorted f sequence_init} 
+-> i: nat { i> 0 && Seq.length sequence_init > (i+1)} 
+-> Tot(r: seq a{Seq.sorted f r})
+
+
+let test #a #f sequence_init i = 
+    let a = Seq.slice sequence_init 0 i in a
+*)
+ val shiftOrderedSequence : #a : eqtype -> #f: (a -> a -> Tot bool) -> 
+                            sequence_init : seq a {Seq.length sequence_init > 0 && Seq.sorted f sequence_init} -> 
+                            i: nat { i> 0 && Seq.length sequence_init > (i+1)} -> 
+                            value: a{
+                            f (Seq.index sequence_init i) value = false  && 
+                            f (Seq.index sequence_init (i+1)) value} -> Tot(r:seq a{Seq.sorted f r})
+let shiftOrderedSequence #a #f sequence_init i value = 
+    let first_part = Seq.slice sequence_init 0 i in (* length = i - 0*)
+    let second_part = Seq.create 1 value in (*length = 1 *)
+    let third_part = Seq.slice sequence_init (i) (Seq.length sequence_init) in (*length = length - i*)
+    sequence_init            
+
+val tl_lemma : #a: eqtype -> #f:(cmp a) -> sequence_init: seq a {Seq.length sequence_init> 1 && Seq.sorted f sequence_init} -> 
+    Lemma(ensures (Seq.sorted f (Seq.tail sequence_init)))
+
+let tl_lemma #a #f sequence_init = ()
+
 val update_indexes: #a: eqtype -> #f: cmp(a) ->sl: skipList a  f -> place:nat {place + 1 < length sl} -> level:nat ->
                         ML(r: seq (non_empty_list nat){Seq.length (getIndexes sl) +1 = Seq.length r  })
 
@@ -127,9 +170,10 @@ assume val searchPlace : #a : eqtype -> #f: cmp(a) ->  comparator: (a-> a -> Tot
             Tot(r: nat {(r+1) < SkipList2.Statement.length sl
                  && comparator (Seq.index (getValues sl) (r-1)) el  = 1 && comparator (Seq.index (getValues sl) (r)) el  = -1})
             
-                    
+*)            (*)    
 assume val inputValue : #a : eqtype -> #f: cmp(a) ->
                     el : a -> sl: skipList a f -> 
                     place : nat{place<SkipList2.Statement.length sl} ->
                     Tot(r:seq a {FStar.Seq.Properties.sorted f r &&
                     Seq.length r = Seq.length(getIndexes sl)+1 })
+let inputValue #a #f el sl place =
